backup.v
@@ -1,0 +1,256 @@
+
+
+
+
+
+
+simpl.
+assert ((n = i + p) \/ (n = S i + p) \/ (n <> i  + p /\ n <> S i + p)).
+omega.
+case H0.
+intros.
+assert (eq_nat_branch n (p + i) (increase_var u p 0)
+  (eq_nat_branch n (p + S i) (increase_var a p 0)
+     (de_bruijn_aux n l p (S (S i)))) = increase_var u p 0).
+apply eq_branch_real_eq.
+omega.
+rewrite H2.
+rewrite neq_branch_real_neq.
+rewrite de_bruijn_aux_terminate.
+simpl.
+apply eq_branch_real_eq.
+trivial.
+omega.
+omega.
+intros.
+case H1.
+intros.
+assert (eq_nat_branch n (p + S i) (increase_var a p 0)
+     (de_bruijn_aux n l p (S (S i))) = increase_var a p 0).
+rewrite eq_branch_real_eq.
+trivial.
+omega.
+rewrite H3.
+assert (eq_nat_branch n (p + i) (increase_var u p 0) (increase_var a p 0) = increase_var a p 0).
+rewrite neq_branch_real_neq.
+trivial.
+omega.
+rewrite H4.
+rewrite missing_variable_substitution.
+trivial.
+simpl in H.
+apply increase_var_keeps_close.
+case H.
+intros.
+trivial.
+intros.
+case H2.
+intros.
+assert (eq_nat_branch n (p + S i) (increase_var a p 0)
+     (de_bruijn_aux n l p (S (S i))) = de_bruijn_aux n l p (S (S i))).
+rewrite neq_branch_real_neq.
+trivial.
+omega.
+rewrite H5.
+assert (eq_nat_branch n (p + i) (increase_var u p 0) (de_bruijn_aux n l p (S (S i))) = de_bruijn_aux n l p (S (S i))).
+rewrite neq_branch_real_neq.
+trivial.
+omega.
+rewrite H6.
+assert (n < i + p \/ n > i + p + 1).
+omega.
+case H7.
+intro.
+rewrite missing_variable_substitution.
+trivial.
+rewrite de_bruijn_aux_terminate.
+simpl.
+trivial.
+omega.
+intro.
+rewrite missing_variable_substitution.
+trivial.
+simpl in IHl.
+
+
+
+
+induction a.
+simpl.
+induction n0.
+rewrite leq_branch_real_leq.
+simpl.
+simpl in H.
+case H.
+intros.
+omega.
+omega.
+simpl.
+simpl in H.
+case H.
+intros.
+omega.
+simpl.
+
+
+
+
+simpl.
+apply closed_implication.
+rewrite nil_substitution in IHt.
+simpl in IHt.
+rewrite nil_subsititution
+rewrite missing_variable_substitution.
+simpl.
+assert ((n = i) \/ (n = S i) \/ (n <> i /\ n <> S i)).
+omega.
+rewrite increase_is_id.
+
+
+
+simpl in IHt.
+
+rewrite IHt.
+assert (de_bruijn_substitution (de_bruijn_substitution_list t nil (S i)) u i = de_bruijn_substitution_list t nil (S i)).
+apply missing_variable_substitution.
+
+
+destruct (beq_nat n i);
+trivial.
+simpl.
+intros.
+rewrite nil_substitution.
+rewrite <- IHt.
+rewrite nil_substitution.
+trivial.
+split.
+apply closed_implication.
+case H.
+trivial.
+trivial.
+intros.
+rewrite nil_substitution.
+simpl.
+rewrite <- IHt1.
+rewrite <- IHt2.
+rewrite nil_substitution.
+rewrite nil_substitution.
+trivial.
+exact H.
+exact H.
+intro.
+induction t.
+intros.
+simpl.
+assert ((n = i) \/ (n = S i) \/ (n <> i /\ n <> S i)).
+omega.
+case H0.
+intro.
+assert (eq_nat_branch n i (increase_var u i 0)
+  (eq_nat_branch n (S i) (increase_var a (S i) 0)
+     (de_bruijn_aux n l (S (S i)))) = increase_var u i 0).
+apply eq_branch_real_eq.
+exact H1.
+rewrite H2.
+assert (eq_nat_branch n (S i) (increase_var a (S i) 0)
+     (de_bruijn_aux n l (S (S i))) = (de_bruijn_aux n l (S (S i)))).
+apply neq_branch_real_neq.
+omega.
+rewrite H3.
+assert (de_bruijn_aux n l (S (S i)) = var n).
+apply de_bruijn_aux_terminate.
+omega.
+rewrite H4.
+simpl.
+apply eq_branch_real_eq.
+exact H1.
+intros.
+case H1.
+intros.
+assert (eq_nat_branch n (S i) (increase_var a (S i) 0)
+     (de_bruijn_aux n l (S (S i))) = increase_var a (S i) 0).
+apply eq_branch_real_eq.
+exact H2.
+rewrite H3.
+assert (eq_nat_branch n i (increase_var u i 0) (increase_var a (S i) 0) = increase_var a (S i) 0).
+apply neq_branch_real_neq.
+omega.
+rewrite H4.
+apply missing_variable_substitution.
+assert (increase_var a (S i) 0 = a).
+apply increase_is_id.
+simpl in H.
+induction a.
+simpl.
+assert (closed i (var n0)).
+case H.
+intros.
+case H6.
+intros.
+trivial.
+simpl in H5.
+
+induction n0.
+assert (gt_nat_branch 0 0 (var (0 + S i)) (var 0) = var 0).
+apply leq_branch_real_leq.
+trivial.
+omega.
+rewrite H6.
+trivial.
+assert (gt_nat_branch (S n0) 0 (var (S n0 + S i)) (var (S n0)) = var (S n0 + S i)).
+apply gt_branch_real_gt.
+omega.
+rewrite H6.
+simpl.
+
+
+case H5.
+induction n0.
+simpl.
+apply closed_implication.
+omega.
+simpl.
+omega.
+intros.
+induction n0.
+simpl.
+omega.
+simpl.
+omega.
+case H.
+intros.
+case H6.
+intros.
+assert (closed (S i) a = closed i (lambda a)).
+simpl.
+trivial.
+simpl.
+
+rewrite H9.
+trivial.
+simpl.
+case H.
+intros.
+case H6.
+intros.
+assert ((closed i a1 /\ closed i a2) = closed i (application a1 a2)).
+simpl.
+trivial.
+rewrite H9.
+trivial.
+intros.
+assert (eq_nat_branch n (S i) (increase_var a (S i) 0)
+     (de_bruijn_aux n l (S (S i))) = de_bruijn_aux n l (S (S i))).
+apply neq_branch_real_neq.
+omega.
+rewrite H3.
+assert (eq_nat_branch n i (increase_var u i 0) (de_bruijn_aux n l (S (S i))) = de_bruijn_aux n l (S (S i))).
+apply neq_branch_real_neq.
+omega.
+rewrite H4.
+apply missing_variable_substitution.
+
+assert (eq_nat_branch n i (increase_var u i 0)
+  (eq_nat_branch n (S i) (increase_var a (S i) 0)
+     (de_bruijn_aux n l (S (S i)))) = de_bruijn_aux n l (S (S i))).
+apply neq_branch_real_neq.
